> # 891.Sum of Subsequence Widths

Tags: `Hard` `math` `sort`

Links: https://leetcode.com/problems/sum-of-subsequence-widths/

----

The **width** of a sequence is the difference between the maximum and minimum elements in the sequence.

Given an array of integers `nums`, return *the sum of the **widths** of all the non-empty **subsequences** of* `nums`. Since the answer may be very large, return it **modulo** `109 + 7`.

A **subsequence** is a sequence that can be derived from an array by deleting some or no elements without changing the order of the remaining elements. For example, `[3,6,2,7]` is a subsequence of the array `[0,3,1,6,2,2,7]`.

 

**Example 1:**

```
Input: nums = [2,1,3]
Output: 6
Explanation: The subsequences are [1], [2], [3], [2,1], [2,3], [1,3], [2,1,3].
The corresponding widths are 0, 0, 0, 1, 1, 2, 2.
The sum of these widths is 6.
```

**Example 2:**

```
Input: nums = [2]
Output: 0
```

 

**Constraints:**

- `1 <= nums.length <= 105`
- `1 <= nums[i] <= 105`

-----

注意此题是子序列而不是子数组，并且只关心最大值和最小值，最开始的时候想到的办法是结合滑动窗口最大值和最小值，然后求得结果，但是时间复杂度为$O(n^2)$。

因为是子序列，所以可以对数组进行排序，对于排序后的数组的第`k`个数字，其前面的`k - 1`个数字可以组成$2^{k - 1} - 1$中组合（去掉空集），在这些组合里面，第`k`个数字始终最为最大值，其对结果的影响是，加入前面某个集合的最大值和最小值为`a, b`，则原有的宽度为`a - b`，加入第`k`个数字后，宽度变为`nums[k - 1] - b = nums[k - 1] - a + a - b`，相当于在原有的基础上增加了$(2^{k - 1} - 1) \times \text{nums}[k - 1]$的数量，反之，第`k`个数字对于右边的子序列的贡献是宽度减少了`nums[k - 1]`。

更加严格的数学证明：

假设`j > i`，对于序列中`nums[j]`和`nums[i]`之间的数字，可以和这两个数字共组成$2 ^ {j - i - 1}$组子序列，于是：
$$
\begin{gathered}
\sum_{j>i}\left(2^{j-i-1}\right)\left(A_{j}-A_{i}\right) \\
=\left(\sum_{i=0}^{n-2} \sum_{j=i+1}^{n-1}\left(2^{j-i-1}\right)\left(A_{j}\right)\right)-\left(\sum_{i=0}^{n-2} \sum_{j=i+1}^{n-1}\left(2^{j-i-1}\right)\left(A_{i}\right)\right) \\
=\left(\sum_{i=0}^{n-2}\left(2^{0}+2^{1}+\cdots+2^{N-i-2}\right)\left(A_{i}\right)\right) \\
=\left(\sum_{j=1}^{n-1}\left(2^{j}-1\right) A_{j}\right)-\left(\sum_{i=0}^{n-2}\left(2^{N-i-1}-1\right) A_{i}\right) \\
=\sum_{i=0}^{n-1}\left(\left(\left(2^{i}-1\right) A_{i}\right)-\left(\left(2^{N-i-1}-1\right) A_{i}\right)\right) \\
\left.\left.A_{2}+2^{2}+\cdots\right)+\left(2^{0} A_{2}+2^{1} A_{3}+\cdots\right)+\left(2^{0} A_{3}+2^{1} A_{4}+\cdots\right)+\cdots\right) \\
=\sum_{i=0}^{n-1}\left(2^{i}-2^{N-i-1}\right) A_{i}
\end{gathered}
$$
所以只需要按照公式计算即可。

```c++
class Solution {
public:
    int sumSubseqWidths(vector<int>& nums) {
    	std::ios_base::sync_with_stdio(false);
    	cin.tie(NULL);
    	cout.tie(NULL);

    	int n = nums.size();
    	const long long MODE = 1e9 + 7;
    	long long res = 0;

        sort(nums.begin(), nums.end());
    	for (int i = 1; i <= n; ++i) {
    		long long addNum = fastPow((long long)2, i - 1, MODE);
    		long long subNum = fastPow((long long)2, n - i, MODE);
    		res = (res + (nums[i - 1] * addNum) % MODE) % MODE;
    		long long tmp = (nums[i - 1] * subNum) % MODE;
    		if (res < tmp) res = (res - tmp + MODE) % MODE;
    		else res = (res - tmp) % MODE;
    	}

    	return res;
    }


    long long fastPow(long long base, int k, const long long & MODE) {
    	long long res = 1;
    	while (k) {
    		if (k & 1) res = ((res % MODE) * (base % MODE)) % MODE;
    		base = (base * base) % MODE;
            k >>= 1;
    	}

    	return res;
    }
};
```

